cfrontend/Cminorgenproof.v
@@ -526,6 +526,27 @@ Proof.
   eauto using match_globalenvs_inject_incr.
 Qed.
 
+Lemma match_globalenvs_wf f hi:
+  match_globalenvs f hi ->
+  CKLR.meminj_wf f.
+Proof.
+  intros [ ]. split.
+  - intros b1 b2 [delta Hb].
+    destruct (Block.ident_of b1) as [i|] eqn:Hb1.
+    * apply Block.ident_of_inv in Hb1; subst.
+      rewrite DOMAIN in Hb; inv Hb. rewrite Block.ident_of_glob; auto.
+      apply Block.lt_le_trans with Block.init; eauto using Block.lt_glob_init.
+      apply Block.le_trans with init_nb; eauto.
+    * destruct (Block.ident_of b2) eqn:Hb2; eauto.
+      rewrite (IMAGE b1 b2 delta Hb) in Hb1; try congruence.
+      eapply Block.ident_of_inv in Hb2; subst.
+      apply Block.lt_le_trans with Block.init; eauto using Block.lt_glob_init.
+      apply Block.le_trans with init_nb; eauto.
+  - intros b b' delta. unfold Mem.flat_inj.
+    destruct Block.lt_dec; inversion 1; subst.
+    eapply DOMAIN. blomega.
+Qed.
+
 (** Invariance properties for [match_callstack]. *)
 
 Lemma match_callstack_invariant:
@@ -2318,11 +2339,8 @@ Proof.
     eapply match_globalenvs_inject_incr; eauto.
   }
   {
-    clear -MCS.
-    apply match_callstack_match_globalenvs in MCS as [hi [ ]].
-    intros b b' delta. unfold Mem.flat_inj.
-    destruct Block.lt_dec; inversion 1; subst.
-    eapply DOMAIN. blomega.
+    eapply match_callstack_match_globalenvs in MCS as [hi Hge].
+    eapply match_globalenvs_wf; eauto.
   }
   inv TR.
   assert (fd = External (EF_external id sg)) by congruence; subst fd.
@@ -2355,6 +2373,7 @@ Proof.
   exists (tv, tm). split.
   - eapply match_reply_cc_inject_triangle; eauto.
     eapply match_globalenvs_inject_incr; eassumption.
+    eapply match_globalenvs_wf; eauto.
   - constructor.
 Qed. 
 
