common/LanguageInterface.v
@@ -188,7 +188,6 @@ Record match_c_query (R: cklr) (w: world R) (q1 q2: c_query) :=
     match_cq_sg: cq_sg q1 = cq_sg q2;
     match_cq_args: list_rel (Val.inject (mi R w)) (cq_args q1) (cq_args q2);
     match_cq_mem: match_mem R w (cq_mem q1) (cq_mem q2);
-    match_cq_valid: inject_incr (Mem.flat_inj Block.init) (mi R w);
   }.
 
 Definition cc_c (R: cklr): callconv li_c li_c :=
@@ -217,13 +216,6 @@ Definition cc_c_tr R: callconv li_c li_c :=
 
 (** *** Extension passes *)
 
-Lemma flat_inject_id_incr thr:
-  inject_incr (Mem.flat_inj thr) inject_id.
-Proof.
-  intros b b' delta. unfold Mem.flat_inj, inject_id.
-  destruct Block.lt_dec; congruence.
-Qed.
-
 Lemma match_cc_ext id sg vargs1 m1 vargs2 m2:
   Mem.extends m1 m2 ->
   Val.lessdef_list vargs1 vargs2 ->
@@ -240,7 +232,6 @@ Proof.
     + exists 0. reflexivity.
     + apply val_inject_list_lessdef in Hvargs.
       induction Hvargs; constructor; eauto.
-    + apply flat_inject_id_incr.
   - intros vres1 m1' vres2 m2' (w' & Hw' & Hvres & Hm'). simpl in *.
     split; auto.
     apply val_inject_lessdef; eauto.
@@ -264,7 +255,6 @@ Proof.
     + apply val_inject_list_lessdef in Hvargs.
       induction Hvargs; constructor; eauto.
     + constructor; eauto.
-    + apply flat_inject_id_incr.
   - intros vres1 m1' vres2 m2' (w' & Hw' & Hvres & Hm'). cbn [fst snd] in *.
     inversion Hw' as [xm1 xm2 xm1' xm2' Hperm Hunch]; subst.
     inv Hm'. simpl in Hvres. red in Hvres.
@@ -278,7 +268,7 @@ Lemma match_cc_inject fb1 sg f vargs1 m1 fb2 vargs2 m2:
   block_inject f fb1 fb2 ->
   Val.inject_list f vargs1 vargs2 ->
   Mem.inject f m1 m2 ->
-  inject_incr (Mem.flat_inj Block.init) f ->
+  meminj_wf f ->
   exists w,
     match_query (cc_c injp) w (cq fb1 sg vargs1 m1) (cq fb2 sg vargs2 m2) /\
     forall vres1 m1' vres2 m2',
@@ -415,7 +405,8 @@ Definition cc_inject_triangle_mr nb: reply li_c -> reply li_c -> Prop :=
     exists f',
       inject_incr (Mem.flat_inj nb) f' /\
       Val.inject f' vres1 vres2 /\
-      Mem.inject f' m1' m2'.
+      Mem.inject f' m1' m2' /\
+      meminj_wf f'.
 
 Definition cc_inject_triangle: callconv li_c li_c :=
   {|
@@ -451,6 +442,7 @@ Lemma match_reply_cc_inject_triangle nb f' vres1 m1' vres2 m2':
   Val.inject f' vres1 vres2 ->
   Mem.inject f' m1' m2' ->
   inject_incr (Mem.flat_inj nb) f' ->
+  meminj_wf f' ->
   match_reply cc_inject_triangle nb (vres1, m1') (vres2, m2').
 Proof.
   intros Hvres Hm' Hf'.
